examples/separationLogic/src/holfoot/holfootSyntax.sig
@@ -3,13 +3,18 @@ sig
 
 include Abbrev;
 
-val holfoot_heap_ty : hol_type;
+val holfoot_heap_ty  : hol_type;
 val holfoot_stack_ty : hol_type;
 val holfoot_state_ty : hol_type;
+val holfoot_var_ty   : hol_type;
+val holfoot_tag_ty   : hol_type;
+val holfoot_a_expression_ty  : hol_type;
+val holfoot_a_proposition_ty : hol_type;
 
 
 val string2holfoot_tag : string -> term
 val string2holfoot_var : string -> term
+val holfoot_var2string : term -> string
 
 val holfoot_mk_call_by_value_arg : (string * term) * term -> term
 val holfoot_mk_const : string -> term
@@ -27,6 +32,7 @@ val holfoot_ap_bintree_term : term
 val holfoot_ap_tree_term : term
 val holfoot_ap_data_tree_term : term
 val holfoot_ap_data_list_seg_term : term
+val holfoot_ap_data_queue_term : term
 val holfoot_ap_data_list_term : term
 val holfoot_ap_eq_cond_term : term
 val holfoot_ap_equal_term : term
@@ -41,6 +47,7 @@ val holfoot_ap_unequal_term : term
 val holfoot_bool_proposition_term : term
 val holfoot_exp_add_term : term
 val holfoot_exp_binop_term : term;
+val holfoot_exp_op_term : term;
 val holfoot_exp_const_term : term
 val holfoot_exp_mult_term : term
 val holfoot_exp_div_term : term
@@ -50,6 +57,7 @@ val holfoot_exp_sub_term : term
 val holfoot_exp_var_term : term
 val holfoot_pred_and_term : term
 val holfoot_pred_bin_term : term
+val holfoot_pred_term : term
 val holfoot_pred_eq_term : term
 val holfoot_pred_false_term : term
 val holfoot_pred_ge_term : term
@@ -79,30 +87,34 @@ val holfoot_var_term  : term
 
 
 val dest_holfoot_ap_bintree : term -> term * term
-val dest_holfoot_ap_tree : term -> term * term
-val dest_holfoot_ap_data_tree : term -> term * term * term
 val dest_holfoot_ap_data_list : term -> term * term * term
 val dest_holfoot_ap_data_list_seg : term -> term * term * term * term
+val dest_holfoot_ap_data_queue : term -> term * term * term * term
+val dest_holfoot_ap_data_tree : term -> term * term * term
+val dest_holfoot_ap_points_to : term -> term * term
+val dest_holfoot_ap_tree : term -> term * term
 val dest_holfoot_prog_dispose : term -> term
 val dest_holfoot_prog_field_assign : term -> term * term * term
 val dest_holfoot_prog_field_lookup : term -> term * term * term
 val dest_holfoot_prog_new : term -> term
+val dest_holfoot_prog_with_resource : term -> term * term * term
 val dest_holfoot_tag : term -> term
 val dest_holfoot_var : term -> term
 val is_holfoot_ap_bintree : term -> bool
-val is_holfoot_ap_tree : term -> bool
-val is_holfoot_ap_data_tree : term -> bool
 val is_holfoot_ap_data_list : term -> bool
 val is_holfoot_ap_data_list_seg : term -> bool
+val is_holfoot_ap_data_queue : term -> bool
+val is_holfoot_ap_data_tree : term -> bool
+val is_holfoot_ap_points_to : term -> bool
+val is_holfoot_ap_tree : term -> bool
+val is_holfoot_exp_null : term -> bool
 val is_holfoot_prog_dispose : term -> bool
 val is_holfoot_prog_field_assign : term -> bool
 val is_holfoot_prog_field_lookup : term -> bool
 val is_holfoot_prog_new : term -> bool
+val is_holfoot_prog_with_resource : term -> bool
 val is_holfoot_tag : term -> bool
 val is_holfoot_var : term -> bool
-val dest_holfoot_ap_points_to : term -> term * term
-val is_holfoot_ap_points_to : term -> bool
-val is_holfoot_exp_null : term -> bool
 
 val holfoot_implies_in_heap_term : term 
 val dest_holfoot_implies_in_heap : term -> term * term * term
