src/list/src/listLib.sig
@@ -7,6 +7,11 @@ sig
 
   (* listSimps *)
   val LIST_ss  : simpLib.ssfrag
+  val LIST_EQ_ss : simpLib.ssfrag
+
+  val NORM_CONS_APPEND_CONV : conv
+  val LIST_EQ_SIMP_CONV : conv
+
   val list_rws : computeLib.compset -> unit
   val list_compset : unit -> computeLib.compset
 
@@ -51,8 +56,5 @@ sig
   val SCANR_CONV : conv -> conv
   val REPLICATE_CONV : conv
   val GENLIST_CONV : conv -> conv
-  val NORM_CONS_APPEND_CONV : conv
 
-  val LIST_EQ_SIMP_CONV : conv
-  val list_eq_simp_ss   : simpLib.ssfrag
 end
