src/parse/kind_pp.sml
@@ -21,9 +21,6 @@ val _ = register_btrace("pp_arity_kinds", pp_arity_kinds)
 fun dest_arity_kind kd = Kind.arity_of kd
        handle HOL_ERR _ => raise ERR "not an arity kind"
 
-val show_kinds = ref 1
-val _ = Feedback.register_trace("kinds", show_kinds, 2)
-
 fun pp_kind0 (G:grammar) backend = let
   fun lookup_kindop s = let
     fun recurse [] = NONE
