src/bag/containerScript.sml
@@ -188,12 +188,23 @@ REPEAT STRIP_TAC THEN
 FULL_SIMP_TAC list_ss [MEM_FILTER] THEN
 METIS_TAC[]);
 
+val CARD_LIST_TO_BAG = Q.store_thm(
+"CARD_LIST_TO_BAG",
+`BAG_CARD (LIST_TO_BAG ls) = LENGTH ls`,
+Induct_on `ls` THEN SRW_TAC [][BAG_CARD_THM,arithmeticTheory.ADD1])
+before export_rewrites ["CARD_LIST_TO_BAG"];
 
-
-
+val BAG_TO_LIST_EQ_NIL = Q.store_thm(
+"BAG_TO_LIST_EQ_NIL",
+`FINITE_BAG b ==>
+ (([] = BAG_TO_LIST b) <=> (b = {||})) /\
+ ((BAG_TO_LIST b = []) <=> (b = {||}))`,
+Q.SPEC_THEN `b` STRUCT_CASES_TAC BAG_cases THEN
+SRW_TAC [][BAG_TO_LIST_THM])
+before export_rewrites ["BAG_TO_LIST_EQ_NIL"];
 
 (*---------------------------------------------------------------------------
-    finate  and bags.
+    finite maps and bags.
  ---------------------------------------------------------------------------*)
 
 val BAG_OF_FMAP = Define `BAG_OF_FMAP f b =
